add `concat` expression + start a proof structure

multiplicities/multiplicities.v
@@ -21,8 +21,9 @@ Fixpoint list_crossproduct {X Y : Type} (lx : list X) (ly : list Y) : list (X*Y)
 
 (***** signatures *****)
 Inductive expr : Type :=
-  | intl : nat -> expr
-  | plus : expr -> expr -> expr.
+  | intl   : nat -> expr
+  | plus   : expr -> expr -> expr
+  | concat : expr -> expr -> expr.
 
 Inductive ty : Type :=
   | intty : ty.
@@ -36,7 +37,7 @@ Inductive mult : Type :=
 Inductive val : Type :=
   | intv : nat -> val.
 
-(***** type check *****)
+(***** type check : expr -> ty *****)
 (* TODO: needs to be a partial function *)
 Fixpoint tc (e : expr) : ty :=
   match e with
@@ -47,13 +48,17 @@ Fixpoint tc (e : expr) : ty :=
       match t1, t2 with
       | intty, intty => intty
       end
+  | concat e1 e2 =>
+      let t1 := tc e1 in
+      let t2 := tc e2 in
+      t1 (* TODO: check equality *)
   end.
 
 Example test_tc_1 :
 tc (plus (intl 1) (intl 2)) = intty.
 Proof. simpl. reflexivity. Qed.
 
-(***** multiplicity check *****)
+(***** multiplicity check : expr -> mult *****)
 (* TODO: lattice as in NaBL2? or keep as function? *)
 Definition mult_crossproduct (m1 : mult) (m2 : mult) : mult :=
   match m1, m2 with
@@ -64,6 +69,15 @@ Definition mult_crossproduct (m1 : mult) (m2 : mult) : mult :=
   | _         , _          => zeroOrMore
   end.
 
+Definition mult_concat (m1 : mult) (m2 : mult) : mult :=
+  match m1, m2 with
+  | oneOrMore, _         => oneOrMore
+  | _        , oneOrMore => oneOrMore
+  | one      , _         => oneOrMore
+  | _        , one       => oneOrMore
+  | _        , _         => zeroOrMore
+  end.
+
 Fixpoint mc (e : expr) : mult :=
   match e with
   | intl _ => one
@@ -71,13 +85,21 @@ Fixpoint mc (e : expr) : mult :=
       let m1 := mc e1 in
       let m2 := mc e2 in
       mult_crossproduct m1 m2
+  | concat e1 e2 =>
+      let m1 := mc e1 in
+      let m2 := mc e2 in
+      mult_concat m1 m2
   end.
 
 Example test_mc_1 :
 mc (plus (intl 1) (intl 2)) = one.
 Proof. simpl. reflexivity. Qed.
 
-(***** interpreter *****)
+Example test_mc_2 :
+mc (concat (intl 1) (intl 2)) = oneOrMore.
+Proof. simpl. reflexivity. Qed.
+
+(***** interpreter : expr -> list val *****)
 Definition eval_plus (v : val * val) : val :=
   match v with
   | (intv n1, intv n2) => intv (n1 + n2)
@@ -91,8 +113,56 @@ Fixpoint eval (b : expr) : list val :=
       let v2 : list val       := eval e2 in
       let vs : list (val*val) := list_crossproduct v1 v2 in
       map eval_plus vs
+  | concat e1 e2 =>
+      let v1 : list val       := eval e1 in
+      let v2 : list val       := eval e2 in
+      v1 ++ v2
   end.
 
 Example test_eval_1 :
 eval (plus (intl 1) (intl 2)) = [intv 3].
 Proof. simpl. reflexivity. Qed.
+
+Example test_eval_2 :
+eval (plus (intl 1) (concat (intl 2) (intl 3))) = [intv 3; intv 4].
+Proof. simpl. reflexivity. Qed.
+
+(***** type of value : list val -> ty *****)
+Definition tv1 (v : val) : ty :=
+  match v with
+  | intv _ => intty
+  end.
+
+(* TODO: 1. how to represent no value? *)
+(* TODO: 2. make partial function, if contains values from different types *)
+Fixpoint tv (vs : list val) : ty :=
+  match vs with
+  | [] => intty (* FIXME: *)
+  | v :: vs => tv1 v (* FIXME: *)
+  end.
+
+(***** multiplicity of value : list val -> mult *****)
+Definition mv (vs : list val) : mult :=
+  match vs with
+  | [] => zeroOrOne
+  | [_] => one
+  | _ => oneOrMore
+  end.
+
+Definition mult_contains (m1 : mult) (m2 : mult) : bool :=
+  match m1, m2 with
+  | zeroOrMore, _         => true
+  | _         , one       => true
+  | zeroOrOne , zeroOrOne => true
+  | oneOrMore , oneOrMore => true
+  | _         , _         => false
+  end.
+
+(***** multiplicity preservation *****)
+Theorem mult_perservation : forall (e : expr),
+  mult_contains (mc e) (mv (eval e)) = true.
+Proof.
+  induction e.
+  - simpl. reflexivity.
+  - simpl.
+Abort. (* here is where the fun starts *)
